theories/interop/wp_prims/write_foreign.v
@@ -48,7 +48,7 @@ Proof using.
   iApply "Hcont". iFrame.
   iApply ("Cont" with "[- $Hpto]"). iFrame.
   rewrite /GC /named. 
-  iExists _, _, _, _, _. iFrame. iPureIntro; split_and!; eauto.
+  repeat iExists _. iFrame. iPureIntro; split_and!; eauto.
   eapply GC_correct_modify_foreign; eauto.
 Qed.
 
