theories/interop/wp_utils.v
@@ -37,159 +37,166 @@ Section RootsRepr.
    roots, and a memr, which are just the rooted cells *)
 Lemma make_repr θ roots_m mem :
     roots_are_live θ roots_m
- -> map_Forall (λ k v, ∃ w , mem !! k = Some (Storing w) ∧ repr_lval θ v w) roots_m
+ -> Forall (map_Forall (λ k v, ∃ w , mem !! k = Some (Storing w) ∧ repr_lval θ v w)) roots_m
  -> ∃ privmem, repr θ roots_m privmem mem.
 Proof.
-  revert mem.
-  induction roots_m as [|l a roots_m Hin IH] using map_ind; intros mem Hlive Hforall.
-  + exists mem, ∅. split_and!.
-    * econstructor.
-    * eapply map_disjoint_empty_r.
-    * by rewrite map_empty_union.
-  + apply map_Forall_insert_1_1 in Hforall as Hforall2.
-    destruct Hforall2 as (w & Hw & Hrep).
-    specialize (IH (delete l mem)).
-    destruct IH as (privmem & memr & IH & Hdisj & Hunion).
-    1: intros l' g Hg; eapply Hlive; rewrite lookup_insert_ne; first done; intros ->; rewrite Hg in Hin; congruence.
-    1: apply map_Forall_lookup; intros i x Hinix;
-       eapply map_Forall_lookup_1 in Hforall.
-    1: destruct Hforall as (w' & H1 & H2); exists w'; repeat split; try done.
-    1: rewrite lookup_delete_ne; first done.
-    2: rewrite lookup_insert_ne; first done.
-    1-2: intros ->; rewrite Hin in Hinix; congruence.
-    assert (memr !! l = None) as HNone1.
-    1: apply not_elem_of_dom; erewrite <- repr_roots_dom; last done; by eapply not_elem_of_dom.
-    assert (privmem !! l = None) as Hnone2.
-    1: rewrite <- (lookup_union_r memr privmem); try done; rewrite <- Hunion; by apply lookup_delete.
-    eexists privmem, (<[l:=Storing w]> memr). split_and!.
-    * econstructor; try done; by eapply not_elem_of_dom.
-    * by apply map_disjoint_insert_r.
-    * erewrite <- insert_union_l. rewrite <- Hunion. rewrite insert_delete_insert.
-      apply map_eq_iff. intros i. destruct (decide (i = l)) as [-> |]; (try by rewrite lookup_insert); by rewrite lookup_insert_ne.
-Qed.
+(*   revert mem. *)
+(*   induction roots_m as [|l a roots_m Hin IH] using map_ind; intros mem Hlive Hforall. *)
+(*   + exists mem, ∅. split_and!. *)
+(*     * econstructor. *)
+(*     * eapply map_disjoint_empty_r. *)
+(*     * by rewrite map_empty_union. *)
+(*   + apply map_Forall_insert_1_1 in Hforall as Hforall2. *)
+(*     destruct Hforall2 as (w & Hw & Hrep). *)
+(*     specialize (IH (delete l mem)). *)
+(*     destruct IH as (privmem & memr & IH & Hdisj & Hunion). *)
+(*     1: intros l' g Hg; eapply Hlive; rewrite lookup_insert_ne; first done; intros ->; rewrite Hg in Hin; congruence. *)
+(*     1: apply map_Forall_lookup; intros i x Hinix; *)
+(*        eapply map_Forall_lookup_1 in Hforall. *)
+(*     1: destruct Hforall as (w' & H1 & H2); exists w'; repeat split; try done. *)
+(*     1: rewrite lookup_delete_ne; first done. *)
+(*     2: rewrite lookup_insert_ne; first done. *)
+(*     1-2: intros ->; rewrite Hin in Hinix; congruence. *)
+(*     assert (memr !! l = None) as HNone1. *)
+(*     1: apply not_elem_of_dom; erewrite <- repr_roots_dom; last done; by eapply not_elem_of_dom. *)
+(*     assert (privmem !! l = None) as Hnone2. *)
+(*     1: rewrite <- (lookup_union_r memr privmem); try done; rewrite <- Hunion; by apply lookup_delete. *)
+(*     eexists privmem, (<[l:=Storing w]> memr). split_and!. *)
+(*     * econstructor; try done; by eapply not_elem_of_dom. *)
+(*     * by apply map_disjoint_insert_r. *)
+(*     * erewrite <- insert_union_l. rewrite <- Hunion. rewrite insert_delete_insert. *)
+(*       apply map_eq_iff. intros i. destruct (decide (i = l)) as [-> |]; (try by rewrite lookup_insert); by rewrite lookup_insert_ne. *)
+(* Qed. *)
+Admitted.
 
 Lemma set_to_none θ mem roots_m privmem :
     repr θ roots_m privmem mem
  -> gen_heap_interp mem
- -∗ ([∗ map] a0↦v0 ∈ roots_m, ∃ w, a0 ↦C{DfracOwn 1} w ∗ ⌜repr_lval θ v0 w⌝)
-==∗ (gen_heap_interp (privmem ∪ ((λ _ : lval, None) <$> roots_m))
-    ∗[∗ set] a0 ∈ dom roots_m, a0 O↦C None).
+ -∗ ([∗ list] r ∈ roots_m, ([∗ map] a0↦v0 ∈ r, ∃ w, a0 ↦C w ∗ ⌜repr_lval θ v0 w⌝))
+==∗ (gen_heap_interp (roots_map_mem' privmem roots_m)
+  ∗ [∗ list] r ∈ roots_m, [∗ set] a0 ∈ dom r, a0 O↦C None).
 Proof.
-  intros (mm & Hrepr1 & Hrepr2 & Hrepr3).
-  induction Hrepr1 in Hrepr2,Hrepr3,mem,privmem|-*.
-  + iIntros "Hheap Hmap !>".
-    rewrite fmap_empty. rewrite dom_empty_L. rewrite map_union_empty.
-    rewrite map_empty_union in Hrepr3. subst mem. iFrame.
-    iApply big_sepS_empty. done.
-  + eapply not_elem_of_dom in H0,H1. iIntros "Hheap Hmap".
-    iPoseProof (big_sepM_insert) as "(Hb1 & _)"; first apply H0.
-    iPoseProof ("Hb1" with "Hmap") as "((%w' & Hw & %Hrepr4) & Hmap)".
-    repr_lval_inj.
-    iMod (gen_heap_update with "Hheap Hw") as "(Hheap & Hw)".
-    specialize (IHHrepr1 (<[a:=None]> mem) (<[a:=None]> privmem)).
-    iMod (IHHrepr1 with "Hheap Hmap") as "(Hheap & Hmap)".
-    * eapply map_disjoint_insert_l_2; first done.
-      erewrite <- (delete_insert mem0); last done.
-      by eapply map_disjoint_delete_r.
-    * subst mem. erewrite <- insert_union_l.
-      rewrite insert_insert. by rewrite insert_union_r.
-    * iModIntro. iSplitL "Hheap".
-      - erewrite <- insert_union_l. rewrite insert_union_r.
-        2: eapply map_disjoint_Some_r; try done; by rewrite lookup_insert.
-        rewrite fmap_insert. iFrame.
-      - rewrite dom_insert_L. iApply big_sepS_insert; first by eapply not_elem_of_dom. iFrame.
-Qed.
+(*   intros (mm & Hrepr1 & Hrepr2 & Hrepr3). *)
+(*   induction Hrepr1 in Hrepr2,Hrepr3,mem,privmem|-*. *)
+(*   + iIntros "Hheap Hmap !>". *)
+(*     rewrite fmap_empty. rewrite dom_empty_L. rewrite map_union_empty. *)
+(*     rewrite map_empty_union in Hrepr3. subst mem. iFrame. *)
+(*     iApply big_sepS_empty. done. *)
+(*   + eapply not_elem_of_dom in H0,H1. iIntros "Hheap Hmap". *)
+(*     iPoseProof (big_sepM_insert) as "(Hb1 & _)"; first apply H0. *)
+(*     iPoseProof ("Hb1" with "Hmap") as "((%w' & Hw & %Hrepr4) & Hmap)". *)
+(*     repr_lval_inj. *)
+(*     iMod (gen_heap_update with "Hheap Hw") as "(Hheap & Hw)". *)
+(*     specialize (IHHrepr1 (<[a:=None]> mem) (<[a:=None]> privmem)). *)
+(*     iMod (IHHrepr1 with "Hheap Hmap") as "(Hheap & Hmap)". *)
+(*     * eapply map_disjoint_insert_l_2; first done. *)
+(*       erewrite <- (delete_insert mem0); last done. *)
+(*       by eapply map_disjoint_delete_r. *)
+(*     * subst mem. erewrite <- insert_union_l. *)
+(*       rewrite insert_insert. by rewrite insert_union_r. *)
+(*     * iModIntro. iSplitL "Hheap". *)
+(*       - erewrite <- insert_union_l. rewrite insert_union_r. *)
+(*         2: eapply map_disjoint_Some_r; try done; by rewrite lookup_insert. *)
+(*         rewrite fmap_insert. iFrame. *)
+(*       - rewrite dom_insert_L. iApply big_sepS_insert; first by eapply not_elem_of_dom. iFrame. *)
+(* Qed. *)
+Admitted.
 
-Lemma repr_roots_repr_lval θ roots m : repr_roots θ roots m -> forall k v, roots !! k = Some v -> exists w, m !! k = Some (Storing w) /\ repr_lval θ v w.
-Proof.
-  induction 1; intros ??.
-  - intros H. rewrite lookup_empty in H. done.
-  - intros [[<- <-]|[Hn1 Hn2]]%lookup_insert_Some.
-    + rewrite lookup_insert. econstructor. done.
-    + rewrite lookup_insert_ne. 2: done. apply IHrepr_roots. done.
-Qed.
+(* FIXME *)
+(* Lemma repr_roots_repr_lval θ roots m : *)
+(*   repr_roots θ roots m -> forall k v, *)
+(*   roots !! k = Some v -> exists w, m !! k = Some (Storing w) /\ repr_lval θ v w. *)
+(* Proof. *)
+(*   induction 1; intros ??. *)
+(*   - intros H. rewrite lookup_empty in H. done. *)
+(*   - intros [[<- <-]|[Hn1 Hn2]]%lookup_insert_Some. *)
+(*     + rewrite lookup_insert. econstructor. done. *)
+(*     + rewrite lookup_insert_ne. 2: done. apply IHrepr_roots. done. *)
+(* Qed. *)
 
 Lemma repr_dom_eq θ mem roots_1 roots_2 p1 p2 m1 m2 :
-   dom roots_1 = dom roots_2
+   map dom roots_1 = map dom roots_2
  → gmap_inj θ
  → repr_raw θ roots_1 p1 mem m1
  → repr_raw θ roots_2 p2 mem m2
  → p1 = p2 ∧ m1 = m2 ∧ roots_1 = roots_2.
 Proof.
-  intros H1 Hinj (Hr1&Hd1&Hu1) (Hr2&Hd2&Hu2).
-  assert (m1 = m2) as ->.
-  { apply repr_roots_dom in Hr1,Hr2. rewrite H1 in Hr1. rewrite Hr1 in Hr2.
-    eapply map_eq_iff. intros i. destruct (m1 !! i) as [v|] eqn:Heq.
-    + eapply elem_of_dom_2 in Heq as Hdom. eapply lookup_union_Some_l in Heq.
-      erewrite <- Hu1 in Heq. erewrite <- Heq. erewrite Hu2.
-      rewrite Hr2 in Hdom.
-      eapply lookup_union_l. apply elem_of_dom in Hdom as [vv Hvv].
-      eapply map_disjoint_Some_l. 1: done. apply Hvv.
-    + symmetry. eapply not_elem_of_dom. rewrite <- Hr2. by eapply not_elem_of_dom. }
-  assert (p1 = p2) as ->.
-  { eapply map_eq_iff. intros i. destruct (p1 !! i) as [v|] eqn:Heq.
-    + eapply elem_of_dom_2 in Heq as Hdom. eapply lookup_union_Some_r in Heq. 2: done.
-      erewrite <- Hu1 in Heq. erewrite <- Heq. erewrite Hu2;
-      eapply lookup_union_r.
-      eapply not_elem_of_dom. eapply map_disjoint_dom in Hd1. set_solver.
-    + destruct (mem !! i) as [v'|] eqn:Heqmem.
-      * pose proof Heqmem as Heq2. rewrite Hu1 in Heqmem.
-        apply lookup_union_Some_inv_l in Heqmem. 2: done. symmetry.
-        eapply map_disjoint_Some_r. 1: done. done.
-      * rewrite Hu2 in Heqmem. apply lookup_union_None_1 in Heqmem. symmetry. apply Heqmem. }
-  split_and!; try done.
-  pose proof (repr_roots_repr_lval _ _ _ Hr2) as Hr2'.
-  clear Hd1 Hu1 Hd2 Hu2 Hr2.
-  induction Hr1 in Hinj, roots_2, H1, Hr2'|-*.
-  { rewrite dom_empty_L in H1. symmetry in H1. apply dom_empty_inv_L in H1. done. }
-  destruct (roots_2 !! a) as [v2|] eqn:Heq.
-  2: { eapply not_elem_of_dom in Heq. rewrite <- H1 in Heq. erewrite dom_insert_L in Heq. set_solver. }
-  erewrite <- (insert_delete roots_2 a v2); last done. f_equiv.
-  - destruct (Hr2' a v2 Heq) as (ww & Heqw & Hrepr).
-    rewrite lookup_insert in Heqw. injection Heqw; intros ->.
-    by eapply repr_lval_inj_1.
-  - eapply IHHr1.
-    + rewrite dom_delete_L. rewrite <- H1. set_solver.
-    + done.
-    + intros k1 v1 [H3 H4]%lookup_delete_Some.
-      destruct (Hr2' _ _ H4) as (ww&[[??]|[? ?]]%lookup_insert_Some&Hww2).
-      1: done.
-      by exists ww.
-Qed.
+(*   intros H1 Hinj (Hr1&Hd1&Hu1) (Hr2&Hd2&Hu2). *)
+(*   assert (m1 = m2) as ->. *)
+(*   { apply repr_roots_dom in Hr1,Hr2. rewrite H1 in Hr1. rewrite Hr1 in Hr2. *)
+(*     eapply map_eq_iff. intros i. destruct (m1 !! i) as [v|] eqn:Heq. *)
+(*     + eapply elem_of_dom_2 in Heq as Hdom. eapply lookup_union_Some_l in Heq. *)
+(*       erewrite <- Hu1 in Heq. erewrite <- Heq. erewrite Hu2. *)
+(*       rewrite Hr2 in Hdom. *)
+(*       eapply lookup_union_l. apply elem_of_dom in Hdom as [vv Hvv]. *)
+(*       eapply map_disjoint_Some_l. 1: done. apply Hvv. *)
+(*     + symmetry. eapply not_elem_of_dom. rewrite <- Hr2. by eapply not_elem_of_dom. } *)
+(*   assert (p1 = p2) as ->. *)
+(*   { eapply map_eq_iff. intros i. destruct (p1 !! i) as [v|] eqn:Heq. *)
+(*     + eapply elem_of_dom_2 in Heq as Hdom. eapply lookup_union_Some_r in Heq. 2: done. *)
+(*       erewrite <- Hu1 in Heq. erewrite <- Heq. erewrite Hu2; *)
+(*       eapply lookup_union_r. *)
+(*       eapply not_elem_of_dom. eapply map_disjoint_dom in Hd1. set_solver. *)
+(*     + destruct (mem !! i) as [v'|] eqn:Heqmem. *)
+(*       * pose proof Heqmem as Heq2. rewrite Hu1 in Heqmem. *)
+(*         apply lookup_union_Some_inv_l in Heqmem. 2: done. symmetry. *)
+(*         eapply map_disjoint_Some_r. 1: done. done. *)
+(*       * rewrite Hu2 in Heqmem. apply lookup_union_None_1 in Heqmem. symmetry. apply Heqmem. } *)
+(*   split_and!; try done. *)
+(*   pose proof (repr_roots_repr_lval _ _ _ Hr2) as Hr2'. *)
+(*   clear Hd1 Hu1 Hd2 Hu2 Hr2. *)
+(*   induction Hr1 in Hinj, roots_2, H1, Hr2'|-*. *)
+(*   { rewrite dom_empty_L in H1. symmetry in H1. apply dom_empty_inv_L in H1. done. } *)
+(*   destruct (roots_2 !! a) as [v2|] eqn:Heq. *)
+(*   2: { eapply not_elem_of_dom in Heq. rewrite <- H1 in Heq. erewrite dom_insert_L in Heq. set_solver. } *)
+(*   erewrite <- (insert_delete roots_2 a v2); last done. f_equiv. *)
+(*   - destruct (Hr2' a v2 Heq) as (ww & Heqw & Hrepr). *)
+(*     rewrite lookup_insert in Heqw. injection Heqw; intros ->. *)
+(*     by eapply repr_lval_inj_1. *)
+(*   - eapply IHHr1. *)
+(*     + rewrite dom_delete_L. rewrite <- H1. set_solver. *)
+(*     + done. *)
+(*     + intros k1 v1 [H3 H4]%lookup_delete_Some. *)
+(*       destruct (Hr2' _ _ H4) as (ww&[[??]|[? ?]]%lookup_insert_Some&Hww2). *)
+(*       1: done. *)
+(*       by exists ww. *)
+(* Qed. *)
+Admitted.
 
 Lemma set_to_some θ mem roots_m privmem :
     repr θ roots_m privmem mem
- -> gen_heap_interp (privmem ∪ ((λ _ : lval, None) <$> roots_m))
- -∗ ([∗ set] a ∈ dom roots_m, a O↦C None)
+ -> gen_heap_interp (roots_map_mem' privmem roots_m)
+ -∗ ([∗ list] r ∈ roots_m, [∗ set] a ∈ dom r, a O↦C None)
  ==∗ gen_heap_interp mem
-     ∗ ([∗ map] a↦v ∈ roots_m, ∃ w, a ↦C{DfracOwn 1} w ∗ ⌜repr_lval θ v w⌝).
+     ∗ ([∗ list] r ∈ roots_m, [∗ map] a↦v ∈ r, ∃ w, a ↦C w ∗ ⌜repr_lval θ v w⌝).
 Proof.
-  intros (mm & Hrepr1 & Hrepr2 & Hrepr3).
-  induction Hrepr1 in Hrepr2,Hrepr3,mem,privmem|-*.
-  + iIntros "Hheap Hset !>".
-    rewrite fmap_empty. rewrite dom_empty_L. rewrite map_union_empty.
-    rewrite map_empty_union in Hrepr3. subst mem. iFrame.
-    iApply big_sepM_empty. done.
-  + eapply not_elem_of_dom in H0,H1. iIntros "Hheap Hset".
-    rewrite dom_insert_L.
-    iPoseProof (big_sepS_insert) as "(Hb1 & _)"; first eapply not_elem_of_dom_2, H0.
-    iPoseProof ("Hb1" with "Hset") as "(Hw & Hset)".
-    rewrite fmap_insert. rewrite <- insert_union_r.
-    2: eapply map_disjoint_Some_r; first done; by rewrite lookup_insert.
-    iMod (gen_heap_update _ _ _ (Storing w) with "Hheap Hw") as "(Hheap & Hw)".
-    rewrite insert_insert.
-    rewrite insert_union_l.
-    iMod (IHHrepr1 with "Hheap Hset") as "(Hheap & Hset)".
-    * eapply map_disjoint_insert_l_2; first done.
-      erewrite <- (delete_insert mem0); last done.
-      by eapply map_disjoint_delete_r.
-    * done.
-    * rewrite <- insert_union_r; last done.
-      subst mem. rewrite insert_union_l. iModIntro.
-      iFrame.
-      iApply (big_sepM_insert_2 with "[Hw] Hset").
-      iExists w. iFrame. done.
-Qed.
+(*   intros (mm & Hrepr1 & Hrepr2 & Hrepr3). *)
+(*   induction Hrepr1 in Hrepr2,Hrepr3,mem,privmem|-*. *)
+(*   + iIntros "Hheap Hset !>". *)
+(*     rewrite fmap_empty. rewrite dom_empty_L. rewrite map_union_empty. *)
+(*     rewrite map_empty_union in Hrepr3. subst mem. iFrame. *)
+(*     iApply big_sepM_empty. done. *)
+(*   + eapply not_elem_of_dom in H0,H1. iIntros "Hheap Hset". *)
+(*     rewrite dom_insert_L. *)
+(*     iPoseProof (big_sepS_insert) as "(Hb1 & _)"; first eapply not_elem_of_dom_2, H0. *)
+(*     iPoseProof ("Hb1" with "Hset") as "(Hw & Hset)". *)
+(*     rewrite fmap_insert. rewrite <- insert_union_r. *)
+(*     2: eapply map_disjoint_Some_r; first done; by rewrite lookup_insert. *)
+(*     iMod (gen_heap_update _ _ _ (Storing w) with "Hheap Hw") as "(Hheap & Hw)". *)
+(*     rewrite insert_insert. *)
+(*     rewrite insert_union_l. *)
+(*     iMod (IHHrepr1 with "Hheap Hset") as "(Hheap & Hset)". *)
+(*     * eapply map_disjoint_insert_l_2; first done. *)
+(*       erewrite <- (delete_insert mem0); last done. *)
+(*       by eapply map_disjoint_delete_r. *)
+(*     * done. *)
+(*     * rewrite <- insert_union_r; last done. *)
+(*       subst mem. rewrite insert_union_l. iModIntro. *)
+(*       iFrame. *)
+(*       iApply (big_sepM_insert_2 with "[Hw] Hset"). *)
+(*       iExists w. iFrame. done. *)
+(* Qed. *)
+Admitted.
 
 End RootsRepr.
 
